Inserters/Unary.dfy
@@ -1,4 +1,4 @@
-module Inserters.Seq{
+module Inserters_Unary{
 
   import opened Circ
   import opened Eval
@@ -8,20 +8,31 @@ module Inserters.Seq{
   import opened ConservedSubcircuit
   import opened MapFunction
 
-  const SeqUFConst := UpdateFunction(
-    1, 1, 1,
-    (si: SI) requires |si.inputs| == 1 && |si.state| == 1 =>
-      SO(si.state, si.inputs))
-
-  function SeqUpdateFunction(): (r: UpdateFunction)
-    ensures r.Valid()
+  function UnaryOp(a: bool, nk: CNodeKind): bool
+    requires CNodeKindIsUnary(nk)
   {
-    reveal UpdateFunction.Valid();
-    SeqUFConst
+    match nk {
+      case CIden =>
+        a
+      case CInv =>
+        !a
+    }
   }
 
-  function InsertSeqImpl(c: Circuit): (r: (Circuit, Scuf))
+  function UnaryUF(nk: CNodeKind): (uf: UpdateFunction)
+    requires CNodeKindIsUnary(nk)
+    ensures uf.Valid()
+  {
+    reveal UpdateFunction.Valid();
+    UpdateFunction(
+      1, 1, 0,
+      (si: SI) requires |si.inputs| == 1 && |si.state| == 0 =>
+        SO([UnaryOp(si.inputs[0], nk)], []))
+  }
+
+  function InsertUnaryImpl(c: Circuit, nk: CNodeKind): (r: (Circuit, Scuf))
     requires c.Valid()
+    requires CNodeKindIsUnary(nk)
     ensures r.0.Valid()
     ensures r.1.SomewhatValid(r.0)
     ensures r.1.MapValid()
@@ -31,20 +42,20 @@ module Inserters.Seq{
     var new_node := GetNewNode(c);
     assert new_node !in c.NodeKind;
     var new_c := Circuit(
-      NodeKind := c.NodeKind[new_node := CSeq],
+      NodeKind := c.NodeKind[new_node := nk],
       PortSource := c.PortSource
     );
     var i_0 := NP(new_node, INPUT_0);
     var o_0 := NP(new_node, OUTPUT_0);
     var inputs := [i_0];
     var outputs := [o_0];
-    var state := [new_node];
+    var state := [];
     var mp := ScufMap(inputs, outputs, state);
     assert mp.Valid() by {
       reveal Seq.HasNoDuplicates();
       reveal Seq.ToSet();
     }
-    var uf := SeqUpdateFunction();
+    var uf := UnaryUF(nk);
     var s := Scuf({new_node}, mp, uf);
     assert s.SomewhatValid(new_c) by {
       reveal Scuf.SomewhatValid();
@@ -57,7 +68,6 @@ module Inserters.Seq{
       reveal AllSeq();
       assert ScValid(new_c, s.sc);
       assert forall np: NP :: np.n in s.sc ==> np !in c.PortSource.Values;
-      assert (AllONPs(new_c, s.sc) >= Seq.ToSet(mp.outputs) >= ConnOutputs(new_c, s.sc));
     }
     assert s.MapValid() by {
       reveal Seq.ToSet();
@@ -66,16 +76,17 @@ module Inserters.Seq{
     (new_c, s)
   }
 
-  lemma InsertSeqF(c: Circuit, fi: FI)
+  lemma InsertUnaryF(c: Circuit, nk: CNodeKind, fi: FI)
     requires c.Valid()
+    requires CNodeKindIsUnary(nk)
     requires
-      var (new_c, s) := InsertSeqImpl(c);
+      var (new_c, s) := InsertUnaryImpl(c, nk);
       FIValid(fi, s.mp.inputs, s.mp.state)
     ensures
-      var (new_c, s) := InsertSeqImpl(c);
+      var (new_c, s) := InsertUnaryImpl(c, nk);
       reveal Scuf.SomewhatValid();
       reveal Seq.ToSet();
-      && s.f(fi) == FO(map[s.mp.outputs[0]:=fi.state[s.mp.state[0]]], map[s.mp.state[0]:=fi.inputs[s.mp.inputs[0]]])
+      && s.f(fi) == FO(map[s.mp.outputs[0]:=UnaryOp(fi.inputs[s.mp.inputs[0]], nk)], map[])
     {
       reveal Scuf.SomewhatValid();
       reveal Seq.ToSet();
@@ -83,43 +94,46 @@ module Inserters.Seq{
       reveal SeqsToMap();
     }
       
-  lemma InsertSeqCorrect(c: Circuit)
+
+
+  lemma InsertUnaryCorrect(c: Circuit, nk: CNodeKind)
     requires c.Valid()
+    requires CNodeKindIsUnary(nk)
     ensures
-      var (new_c, e) := InsertSeqImpl(c);
+      var (new_c, e) := InsertUnaryImpl(c, nk);
       && e.Valid(new_c)
   {
-    var (new_c, e) := InsertSeqImpl(c);
+    var (new_c, e) := InsertUnaryImpl(c, nk);
     var o := e.mp.outputs[0];
-    var st := e.mp.state[0];
     var i_0 := e.mp.inputs[0];
     var path := [e.mp.outputs[0]];
     assert PathValid(new_c, path) && PathValid(new_c, [o, i_0]) by {
       reveal PathValid();
     }
-    var os_0 := NP(e.mp.state[0], OUTPUT_0);
     LengthOneNoDuplicates(path);
     assert new_c.Valid();
     reveal Seq.ToSet();
     forall fi: FI | FIValid(fi, e.mp.inputs, e.mp.state)
       ensures
         var iv_0 := fi.inputs[i_0];
-        var sv_0 := fi.state[i_0.n];
         && FICircuitValid(new_c, fi)
-        && (EvaluateONP(new_c, o, fi) == EvalOk(sv_0))
+        && (EvaluateONP(new_c, o, fi) == EvalOk(UnaryOp(iv_0, nk)))
     {
       var iv_0 := fi.inputs[i_0];
-      var sv_0 := fi.state[os_0.n];
       assert Seq.HasNoDuplicates(path);
       assert FICircuitValid(new_c, fi) by {
         reveal UpdateFunction.Valid();
         reveal FICircuitValid();
       }
-      assert EvaluateONP(new_c, o, fi) == EvalOk(sv_0);
+      assert EvaluateONP(new_c, o, fi) == EvaluateONPUnary(new_c, [o], fi);
       reveal Seq.HasNoDuplicates();
-      assert Evaluate(new_c, o, fi) == EvalOk(sv_0);
+      assert EvaluateINPInner(new_c, [o, i_0], fi) == EvalOk(iv_0);
+      assert EvaluateONPUnary(new_c, [o], fi) == EvalOk(UnaryOp(iv_0, nk));
+      assert EvaluateONPInner(new_c, [o], fi) == EvalOk(UnaryOp(iv_0, nk));
+      assert EvaluateONP(new_c, o, fi) == EvalOk(UnaryOp(iv_0, nk));
+      assert Evaluate(new_c, o, fi) == EvalOk(UnaryOp(iv_0, nk));
       assert Evaluate(new_c, o, fi) == EvalOk(e.f(fi).outputs[o]) by {
-        reveal MapMatchesSeqs();
+        InsertUnaryF(c, nk, fi);
       }
     }
     assert ScValid(new_c, e.sc) by {
@@ -132,17 +146,18 @@ module Inserters.Seq{
     assert e.Valid(new_c);
   }
 
-  lemma InsertSeqConserves(c: Circuit)
+  lemma InsertUnaryConserves(c: Circuit, nk: CNodeKind)
     requires c.Valid()
-    ensures CircuitConserved(c, InsertSeqImpl(c).0)
-    ensures CircuitUnconnected(c, InsertSeqImpl(c).0)
+    requires CNodeKindIsUnary(nk)
+    ensures CircuitConserved(c, InsertUnaryImpl(c, nk).0)
+    ensures CircuitUnconnected(c, InsertUnaryImpl(c, nk).0)
     ensures
-      var (new_c, e) := InsertSeqImpl(c);
+      var (new_c, e) := InsertUnaryImpl(c, nk);
       IsIsland(new_c, e.sc)
   {
     reveal CircuitConserved();
     reveal CircuitUnconnected();
-    var (new_c, e) := InsertSeqImpl(c);
+    var (new_c, e) := InsertUnaryImpl(c, nk);
     reveal Circuit.Valid();
     assert (forall np :: np in c.PortSource.Keys ==> np.n !in e.sc);
     assert (forall np :: np in c.PortSource.Values ==> np.n !in e.sc);
@@ -151,30 +166,33 @@ module Inserters.Seq{
     reveal IsIsland();
   }
 
-  function InsertSeq(c: Circuit): (r: (Circuit, Scuf))
+  function InsertUnary(c: Circuit, nk: CNodeKind): (r: (Circuit, Scuf))
     requires c.Valid()
+    requires CNodeKindIsUnary(nk)
     ensures
       var (new_c, e) := r;
-      && r == InsertSeqImpl(c)
+      && r == InsertUnaryImpl(c, nk)
       && r.0.Valid()
       && e.Valid(new_c)
       && CircuitConserved(c, r.0)
       && CircuitUnconnected(c, r.0)
       && IsIsland(new_c, e.sc)
   {
-    InsertSeqCorrect(c);
-    InsertSeqConserves(c);
-    InsertSeqImpl(c)
+    InsertUnaryCorrect(c, nk);
+    InsertUnaryConserves(c, nk);
+    InsertUnaryImpl(c, nk)
   }
 
-  const SeqInserterConst := ScufInserter(SeqUpdateFunction(), InsertSeq)
-
-  function SeqInserter(): (r: ScufInserter)
+  function UnaryInserter(nk: CNodeKind): (r: ScufInserter)
+    requires CNodeKindIsUnary(nk)
     ensures r.Valid()
   {
     reveal UpdateFunction.Valid();
     reveal ScufInserter.Valid();
-    var z := SeqInserterConst;
+    var z := ScufInserter(
+      UnaryUF(nk),
+      (c: Circuit) requires c.Valid() => InsertUnary(c, nk)
+      );
     assert z.Valid() by {
       reveal SimpleInsertion();
     }
