Inserters/Binary.dfy
@@ -1,0 +1,208 @@
+module Inserters_Binary {
+
+  import opened Circ
+  import opened Scuf 
+  import opened MapFunction
+  import opened Subcircuit
+  import opened Utils
+  import opened Eval
+  import opened ConservedSubcircuit
+
+  function BinaryOp(a: bool, b: bool, nk: CNodeKind): bool
+    requires CNodeKindIsBinary(nk)
+  {
+    match nk {
+      case CAnd =>
+        a && b
+      case COr =>
+        a || b
+      case CXor =>
+        Xor(a, b)
+    }
+  }
+
+  function BinaryUF(nk: CNodeKind): (uf: UpdateFunction)
+    requires CNodeKindIsBinary(nk)
+    ensures uf.Valid()
+  {
+    reveal UpdateFunction.Valid();
+    UpdateFunction(
+      2, 1, 0,
+      (si: SI) requires |si.inputs| == 2 && |si.state| == 0
+        => SO([BinaryOp(si.inputs[0], si.inputs[1], nk)], [])
+    )
+  }
+
+  function InsertBinaryImpl(c: Circuit, nk: CNodeKind): (r: (Circuit, Scuf))
+    requires c.Valid()
+    requires CNodeKindIsBinary(nk)
+    ensures r.0.Valid()
+    ensures r.1.SomewhatValid(r.0)
+    ensures r.1.MapValid()
+    ensures r.1.uf.Valid()
+  {
+    reveal Circuit.Valid();
+    var new_node := GetNewNode(c);
+    assert new_node !in c.NodeKind;
+    var new_c := Circuit(
+      NodeKind := c.NodeKind[new_node := nk],
+      PortSource := c.PortSource
+    );
+    var i_0 := NP(new_node, INPUT_0);
+    var i_1 := NP(new_node, INPUT_1);
+    var o_0 := NP(new_node, OUTPUT_0);
+    var inputs := [i_0, i_1];
+    var outputs := [o_0];
+    var state := [];
+    var mp := ScufMap(inputs, outputs, state);
+    assert mp.Valid() by {
+      reveal Seq.HasNoDuplicates();
+      reveal Seq.ToSet();
+    }
+    var uf := BinaryUF(nk);
+    var s := Scuf({new_node}, mp, uf);
+    assert s.SomewhatValid(new_c) by {
+      reveal Scuf.SomewhatValid();
+      reveal Seq.ToSet();
+      reveal ScValid();
+      reveal ConnOutputs();
+      reveal ConnInputs();
+      reveal UnconnInputs();
+      reveal AllONPs();
+      reveal AllSeq();
+      assert ScValid(new_c, s.sc);
+      assert forall np: NP :: np.n in s.sc ==> np !in c.PortSource.Values;
+    }
+    assert s.MapValid() by {
+      reveal Seq.ToSet();
+      reveal NPsInSc();
+    }
+    (new_c, s)
+  }
+
+  lemma InsertBinaryF(c: Circuit, nk: CNodeKind, fi: FI)
+    requires c.Valid()
+    requires CNodeKindIsBinary(nk)
+    requires
+      var (new_c, s) := InsertBinaryImpl(c, nk);
+      FIValid(fi, s.mp.inputs, s.mp.state)
+    ensures
+      var (new_c, s) := InsertBinaryImpl(c, nk);
+      reveal Scuf.SomewhatValid();
+      reveal Seq.ToSet();
+      && s.f(fi) == FO(map[s.mp.outputs[0]:=BinaryOp(fi.inputs[s.mp.inputs[0]], fi.inputs[s.mp.inputs[1]], nk)], map[])
+    {
+      reveal Scuf.SomewhatValid();
+      reveal Seq.ToSet();
+      reveal MapToSeq();
+      reveal SeqsToMap();
+    }
+
+  lemma InsertBinaryCorrect(c: Circuit, nk: CNodeKind)
+    requires c.Valid()
+    requires CNodeKindIsBinary(nk)
+    ensures
+      var (new_c, s) := InsertBinaryImpl(c, nk);
+      && s.Valid(new_c)
+  {
+    var (new_c, s) := InsertBinaryImpl(c, nk);
+    var o := s.mp.outputs[0];
+    var i_0 := s.mp.inputs[0];
+    var i_1 := s.mp.inputs[1];
+    var path := [s.mp.outputs[0]];
+    assert PathValid(new_c, path) && PathValid(new_c, [o, i_0]) && PathValid(new_c, [o, i_1]) by {
+      reveal PathValid();
+    }
+    LengthOneNoDuplicates(path);
+    assert new_c.Valid();
+    reveal Seq.ToSet();
+    forall fi: FI | FIValid(fi, s.mp.inputs, s.mp.state)
+      ensures
+        var iv_0 := fi.inputs[i_0];
+        var iv_1 := fi.inputs[i_1];
+        && FICircuitValid(new_c, fi)
+        && (EvaluateONP(new_c, o, fi) == EvalOk(BinaryOp(iv_0, iv_1, nk)))
+    {
+      var iv_0 := fi.inputs[i_0];
+      var iv_1 := fi.inputs[i_1];
+      assert Seq.HasNoDuplicates(path);
+      assert FICircuitValid(new_c, fi) by {
+        reveal UpdateFunction.Valid();
+        reveal FICircuitValid();
+      }
+      assert EvaluateONP(new_c, o, fi) == EvaluateONPBinary(new_c, [o], fi);
+      reveal Seq.HasNoDuplicates();
+      assert EvaluateINPInner(new_c, [o, i_0], fi) == EvalOk(iv_0);
+      assert EvaluateINPInner(new_c, [o, i_1], fi) == EvalOk(iv_1);
+      assert EvaluateONPBinary(new_c, [o], fi) == EvalOk(BinaryOp(iv_0, iv_1, nk));
+      assert EvaluateONPInner(new_c, [o], fi) == EvalOk(BinaryOp(iv_0, iv_1, nk));
+      assert EvaluateONP(new_c, o, fi) == EvalOk(BinaryOp(iv_0, iv_1, nk));
+      assert Evaluate(new_c, o, fi) == EvalOk(BinaryOp(iv_0, iv_1, nk));
+      assert Evaluate(new_c, o, fi) == EvalOk(s.f(fi).outputs[o]) by {
+        InsertBinaryF(c, nk, fi);
+      }
+    }
+    assert ScValid(new_c, s.sc) by {
+      reveal Scuf.SomewhatValid();
+    }
+    assert s.EvaluatesCorrectly(new_c) by {
+      reveal Scuf.EvaluatesCorrectly();
+      reveal MapMatchesSeqs();
+    }
+    assert s.Valid(new_c);
+  }
+
+  lemma InsertBinaryConserves(c: Circuit, nk: CNodeKind)
+    requires c.Valid()
+    requires CNodeKindIsBinary(nk)
+    ensures CircuitConserved(c, InsertBinaryImpl(c, nk).0)
+    ensures CircuitUnconnected(c, InsertBinaryImpl(c, nk).0)
+    ensures
+      var (new_c, e) := InsertBinaryImpl(c, nk);
+      IsIsland(new_c, e.sc)
+  {
+    reveal CircuitConserved();
+    reveal CircuitUnconnected();
+    var (new_c, e) := InsertBinaryImpl(c, nk);
+    reveal Circuit.Valid();
+    assert (forall np :: np in c.PortSource.Keys ==> np.n !in e.sc);
+    assert (forall np :: np in c.PortSource.Values ==> np.n !in e.sc);
+    assert (forall np :: np in new_c.PortSource && np.n in e.sc ==> new_c.PortSource[np].n in e.sc);
+    assert (forall np :: np in new_c.PortSource && np.n !in e.sc ==> new_c.PortSource[np].n !in e.sc);
+    reveal IsIsland();
+  }
+
+  function InsertBinary(c: Circuit, nk: CNodeKind): (r: (Circuit, Scuf))
+    requires c.Valid()
+    requires CNodeKindIsBinary(nk)
+    ensures
+      var (new_c, e) := r;
+      && r == InsertBinaryImpl(c, nk)
+      && r.0.Valid()
+      && e.Valid(new_c)
+      && CircuitConserved(c, r.0)
+      && CircuitUnconnected(c, r.0)
+      && IsIsland(new_c, e.sc)
+  {
+    InsertBinaryCorrect(c, nk);
+    InsertBinaryConserves(c, nk);
+    InsertBinaryImpl(c, nk)
+  }
+  
+  function BinaryInserter(nk: CNodeKind): (r: ScufInserter)
+    requires CNodeKindIsBinary(nk)
+    ensures r.Valid()
+  {
+    reveal UpdateFunction.Valid();
+    reveal ScufInserter.Valid();
+    var z := ScufInserter(
+      BinaryUF(nk),
+      (c: Circuit) requires c.Valid() => InsertBinary(c, nk)
+      );
+    assert z.Valid() by {
+      reveal SimpleInsertion();
+    }
+    z 
+  }
+
+}
