Inserters/Inv.dfy
@@ -1,4 +1,4 @@
-module Inserters.Ident {
+module Inserters.Inv{
 
   import opened Circ
   import opened ConservedSubcircuit
@@ -6,23 +6,23 @@ module Inserters.Ident {
   import opened Inserters_Unary
   import opened Modifiers.SwitchUF
 
-  function IdentUF(): (r: UpdateFunction)
+  function InvUF(): (r: UpdateFunction)
     ensures r.Valid()
   {
     reveal UpdateFunction.Valid();
     UpdateFunction(
       1, 1, 0,
       (si: SI) requires |si.inputs| == 1 && |si.state| == 0 =>
-        SO([si.inputs[0]], [])
+        SO([!si.inputs[0]], [])
       )
   }
 
-  function IdentInserter(): (z: ScufInserter)
+  function InvInserter(): (z: ScufInserter)
     ensures z.Valid()
   {
-    var z_binary := UnaryInserter(CIden);
+    var z_binary := UnaryInserter(CInv);
     reveal UpdateFunctionsEquiv();
-    var z := SwitchUFModifier(z_binary, IdentUF());
+    var z := SwitchUFModifier(z_binary, InvUF());
     z
   }
 
