Modifiers/ForwardConnect.dfy
@@ -1,0 +1,595 @@
+module Inserters.ForwardConnect{
+
+  import opened Std.Wrappers
+
+  import opened Circ
+  import opened Eval
+  import opened ConservedSubcircuit
+  import opened Utils
+  import opened Scuf
+  import opened MapFunction
+  import opened ConnectionEval
+  import opened Connection
+  import opened Subcircuit
+  import opened MapConnection
+  import opened Modifiers.Merge
+  import opened SelfConnect
+  import opened Modifiers.Connect
+  import opened Path
+  import opened Modifiers.SwitchUF
+  import opened Modifiers.NewOutputs
+
+
+  function ForwardConnectSF(uf1: UpdateFunction, uf2: UpdateFunction, conn: InternalConnection, si: SI): (so: SO)
+    // Here the connection is mapping the uf1.outputs and the left over inputs to the uf2 inputs.
+    requires uf1.Valid()
+    requires uf2.Valid()
+    requires conn.Valid()
+    requires conn.i_width == uf2.input_width
+    requires conn.o_width == uf1.output_width
+    requires |si.inputs| == uf1.input_width + conn.ni_width
+    requires |si.state| == uf1.state_width + uf2.state_width
+  {
+    reveal UpdateFunction.Valid();
+    var si1: SI := SI(si.inputs[..uf1.input_width], si.state[..uf1.state_width]);
+    var so1 := uf1.sf(si1);
+    var si2_true_input := si.inputs[uf1.input_width..];
+    var si2_input := conn.NIO2I(si2_true_input, so1.outputs);
+    var si2 := SI(si2_input, si.state[uf1.state_width..]);
+    var so2 := uf2.sf(si2);
+    var so := SO(so1.outputs + so2.outputs, so1.state + so2.state);
+    so
+  }
+
+  function ForwardConnectUF(uf1: UpdateFunction, uf2: UpdateFunction, conn: InternalConnection): (new_uf: UpdateFunction)
+    requires uf1.Valid()
+    requires uf2.Valid()
+    requires conn.Valid()
+    requires conn.i_width == uf2.input_width
+    requires conn.o_width == uf1.output_width
+    ensures new_uf.Valid()
+  {
+    reveal UpdateFunction.Valid();
+    UpdateFunction(
+      uf1.input_width + conn.ni_width, uf1.output_width + uf2.output_width, uf1.state_width + uf2.state_width,
+      (si: SI) requires |si.inputs| == uf1.input_width + conn.ni_width && |si.state| == uf1.state_width + uf2.state_width =>
+        ForwardConnectSF(uf1, uf2, conn, si)
+        )
+  }
+
+  function hack(b: bool, n: nat): (bool, nat)
+    // Just to get around dafny's struggles width seq<(bool, int)> vs seq<(bool, nat)>.
+  {
+    (b, n)
+  }
+
+  opaque function NewI2NI(input_width_1: nat, ni_width: nat, i2ni: seq<nat>): (new_i2ni: seq<nat>)
+    requires Seq.HasNoDuplicates(i2ni)
+    requires |i2ni| == ni_width - input_width_1
+    ensures Seq.HasNoDuplicates(new_i2ni)
+    ensures |new_i2ni| == ni_width
+  {
+    reveal Seq.HasNoDuplicates();
+    var i2ni := seq(ni_width, (i: nat) requires i < ni_width =>
+                if i < input_width_1 then i else i2ni[i-input_width_1] + input_width_1);
+    i2ni
+  }
+
+  lemma NewNIO2IProperties(input_width_1:  nat, input_width_2: nat, nio2i: seq<(bool, nat)>, index: nat)
+    requires Seq.HasNoDuplicates(nio2i)
+    requires |nio2i| == input_width_2
+    requires index < input_width_1 + input_width_2
+    ensures
+      var new_nio2i := NewNIO2I(input_width_1, input_width_2, nio2i);
+      && (index < input_width_1 ==> new_nio2i[index] == (false, index))
+      && (index >= input_width_1 ==> (
+        var (from_output, other_index) := nio2i[index-input_width_1];
+        && (from_output ==> (
+          && new_nio2i[index] == (true, other_index))
+          )
+        && (!from_output ==> new_nio2i[index] == (false, other_index + input_width_1))
+        && (from_output == new_nio2i[index].0)
+      ))
+  {
+    reveal NewNIO2I();
+    if index >= input_width_1 {
+      var (from_output, other_index) := nio2i[index-input_width_1];
+    }
+  }
+
+  opaque function NewNIO2I(input_width_1: nat, input_width_2: nat, nio2i: seq<(bool, nat)>): (new_nio2i: seq<(bool, nat)>)
+    requires Seq.HasNoDuplicates(nio2i)
+    requires |nio2i| == input_width_2
+    ensures Seq.HasNoDuplicates(new_nio2i)
+    ensures |new_nio2i| == input_width_1 + input_width_2
+  {
+    reveal Seq.HasNoDuplicates();
+    var i_width := input_width_1 + input_width_2;
+    var new_nio2i: seq<(bool, nat)> := seq(i_width, (i: nat) requires i < i_width =>
+                if i < input_width_1 then hack(false, i) else
+                  var (from_output, index) := nio2i[i-input_width_1];
+                  if from_output then hack(true, index) else hack(false, index +input_width_1));
+    assert Seq.HasNoDuplicates(new_nio2i) by {
+      forall i1: nat, i2: nat | i1 != i2 && i1 < i_width && i2 < i_width
+        ensures new_nio2i[i1] != new_nio2i[i2]
+      {
+        if i1 < input_width_1 {
+          if i2 < input_width_1 {
+            assert new_nio2i[i1] != new_nio2i[i2];
+          } else {
+            var (from_output, index) := nio2i[i2-input_width_1];
+            assert new_nio2i[i1] != new_nio2i[i2];
+          }
+        } else {
+          var (from_output1, index1) := nio2i[i1-input_width_1];
+          if i2 < input_width_1 {
+            assert new_nio2i[i1] != new_nio2i[i2];
+          } else {
+            var (from_output2, index2) := nio2i[i2-input_width_1];
+            assert new_nio2i[i1] != new_nio2i[i2];
+          }
+        }
+      }
+    }
+    new_nio2i
+  }
+
+  opaque function NewConnections(input_width_1: nat, connections: map<nat, nat>): (new_connections: map<nat, nat>)
+    ensures new_connections.Values == connections.Values
+  {
+    var new_connections := (map k | k in connections ::
+      (k + input_width_1) := connections[k]);
+    assert new_connections.Values == connections.Values by {
+      forall v | v in new_connections.Values
+        ensures v in connections.Values
+      {
+      }
+      forall v | v in connections.Values
+        ensures v in new_connections.Values
+      {
+        var k: nat :| k in connections && connections[k] == v;
+        var new_k := k + input_width_1;
+        assert new_connections[new_k] == v;
+      }
+    }
+    new_connections
+  }
+
+  lemma NewConnectionsHelper2(input_width_1: nat, connections: map<nat, nat>, forward_index: nat)
+    requires forward_index !in connections
+    ensures
+      var new_connections := NewConnections(input_width_1, connections);
+      && forward_index + input_width_1 !in new_connections
+  {
+    reveal NewConnections();
+  }
+
+  lemma NewConnectionsHelper(input_width_1: nat, output_width_1: nat, connections: map<nat, nat>,
+                             forward_index: nat)
+    requires forall o_index :: o_index in connections.Values ==> o_index < output_width_1
+    requires forward_index in connections
+    ensures
+      var new_connections := NewConnections(input_width_1, connections);
+      && forward_index + input_width_1 in new_connections
+      && new_connections[forward_index + input_width_1] == connections[forward_index]
+  {
+    reveal NewConnections();
+  }
+
+  lemma NewConnectionsProperties(input_width_1: nat, output_width_1: nat, connections: map<nat, nat>)
+    requires forall o_index :: o_index in connections.Values ==> o_index < output_width_1
+    ensures
+      var new_connections := NewConnections(input_width_1, connections);
+      && (forall o_index :: o_index in new_connections.Values ==> o_index < output_width_1)
+      && (forall i_index :: i_index in new_connections.Keys ==> i_index >= input_width_1)
+      && forall forward_index :: forward_index in connections ==> forward_index + input_width_1 in new_connections
+  {
+    reveal NewConnections();
+    reveal InternalConnection.ConnectionsValid();
+    var new_connections := NewConnections(input_width_1, connections);
+    assert forall o_index :: o_index in new_connections.Values ==> o_index < output_width_1;
+    assert new_connections.Values == connections.Values;
+  }
+
+  lemma InternalConnectionToIMapValid(uf1: UpdateFunction, uf2: UpdateFunction, forward_conn: InternalConnection)
+    requires uf1.Valid()
+    requires uf2.Valid()
+    requires forward_conn.Valid()
+    requires forward_conn.i_width == uf2.input_width
+    requires forward_conn.o_width == uf1.output_width
+    ensures
+      var internal_conn := ForwardConnectionToInternalConnectionImpl(uf1, uf2, forward_conn);
+      internal_conn.ToIMapValid()
+  {
+    var internal_conn := ForwardConnectionToInternalConnectionImpl(uf1, uf2, forward_conn);
+    var i_width := internal_conn.i_width;
+    var ni_width := internal_conn.ni_width;
+    var o_width := internal_conn.o_width;
+    var nio2i := internal_conn.nio2i;
+    var connections := internal_conn.connections;
+    var i2ni := internal_conn.i2ni;
+
+    assert connections == NewConnections(uf1.input_width, forward_conn.connections);
+
+    forall i_index: nat | i_index < i_width
+      ensures
+        var (from_output, index) := nio2i[i_index];
+        && ((!from_output) ==> index < ni_width && i2ni[index] == i_index && (i_index !in connections))
+        && ((from_output) ==> index < o_width && (i_index in connections) && (index == connections[i_index]))
+    {
+      var (from_output, index) := nio2i[i_index];
+      assert forall o_index :: o_index in forward_conn.connections.Values
+               ==> o_index < uf1.output_width by {
+        reveal InternalConnection.ConnectionsValid();
+      }
+      NewConnectionsProperties(uf1.input_width, uf1.output_width, forward_conn.connections);
+      NewNIO2IProperties(uf1.input_width, uf2.input_width, forward_conn.nio2i, i_index);
+      if i_index < uf1.input_width {
+        //NIO2IHelper1(uf1.input_width, uf2.input_width, forward_conn.nio2i, i_index);
+        assert !from_output;
+        assert index == i_index;
+        assert i2ni[index] == i_index by {
+          reveal NewI2NI();
+        }
+        assert i_index !in connections;
+      } else {
+        var i_index_in_2 := i_index - uf1.input_width;
+        var (forward_from_output, forward_index) := forward_conn.nio2i[i_index_in_2];
+        assert from_output == forward_from_output;
+        if from_output {
+          reveal InternalConnection.ToIMapValid();
+          assert forward_index < uf1.output_width by {
+            assert forward_from_output;
+          }
+          assert index < o_width;
+          assert index == forward_index;
+          assert i_index_in_2 in forward_conn.connections by {
+            reveal InternalConnection.ConnectionsValid();
+          }
+          NewConnectionsHelper(uf1.input_width, uf1.output_width, forward_conn.connections, i_index_in_2);
+          assert (i_index in connections);
+          assert (forward_index == forward_conn.connections[i_index_in_2]);
+          assert (index == connections[i_index]) by {
+            reveal InternalConnection.ConnectionsValid();
+            NewConnectionsHelper(uf1.input_width, uf1.output_width, forward_conn.connections, i_index_in_2);
+            assert i_index_in_2 + uf1.input_width in connections;
+          }
+        } else {
+          // We know that:
+          // var (from_output, index) := nio2i[i_index];
+          // var (forward_from_output, forward_index) := forward_conn.nio2i[i_index - uf1.input_width];
+          assert forward_index == index - uf1.input_width by {
+            reveal NewNIO2I();
+          } 
+          assert forward_index < ni_width - uf1.input_width by {
+            reveal InternalConnection.ToIMapValid();
+          }
+          assert index < ni_width;
+          assert i2ni[index] == i_index &&
+                 forward_conn.i2ni[index - uf1.input_width] == i_index - uf1.input_width by {
+            reveal InternalConnection.ToNIMapValid();
+            reveal InternalConnection.ToIMapValid();
+            reveal NewI2NI();
+            assert i2ni[index] == i_index;
+          }
+          assert (i_index !in connections) by {
+            reveal InternalConnection.ToIMapValid();
+            reveal InternalConnection.ToNIMapValid();
+            assert i_index_in_2 !in forward_conn.connections;
+            reveal NewConnections();
+            NewConnectionsHelper2(uf1.input_width, forward_conn.connections, i_index_in_2);
+            assert connections == NewConnections(uf1.input_width, forward_conn.connections);
+            assert i_index_in_2 + uf1.input_width !in connections;
+          }
+        }
+      }
+    }
+    reveal InternalConnection.ToIMapValid();
+  }
+
+  function ForwardConnectionToInternalConnectionImpl(
+    uf1: UpdateFunction, uf2: UpdateFunction, forward_conn: InternalConnection): (internal_conn: InternalConnection)
+    requires uf1.Valid()
+    requires uf2.Valid()
+    requires forward_conn.Valid()
+    requires forward_conn.i_width == uf2.input_width
+    requires forward_conn.o_width == uf1.output_width
+    ensures internal_conn.BasicValid()
+  {
+    var ni_width := uf1.input_width + forward_conn.ni_width;
+    var i_width := uf1.input_width + uf2.input_width;
+    var o_width := uf1.output_width + uf2.output_width;
+    // For the connections the keys are now pointing at the combined inputs and must be increases by uf1.input_width
+    // The values are pointing at combined outputs but are unchanged.
+    var connections := NewConnections(uf1.input_width, forward_conn.connections);
+    var i2ni := NewI2NI(uf1.input_width, ni_width, forward_conn.i2ni);
+    var nio2i := NewNIO2I(uf1.input_width, uf2.input_width, forward_conn.nio2i);
+    var internal_conn := InternalConnection(ni_width, i_width, o_width, connections, i2ni, nio2i);
+    reveal Seq.HasNoDuplicates();
+    assert (ni_width <= i_width);
+    assert (i_width <= ni_width + o_width);
+    assert (|i2ni| == ni_width);
+    assert (|nio2i| == i_width);
+    assert Seq.HasNoDuplicates(i2ni);
+    assert Seq.HasNoDuplicates(nio2i);
+    internal_conn
+  }
+
+  function ForwardConnectionToInternalConnection(
+      uf1: UpdateFunction, uf2: UpdateFunction, forward_conn: InternalConnection): (internal_conn: InternalConnection)
+    // Transform a connection that is connection uf1 outputs to uf2 inputs to a connection that is connecting
+    // the merged outputs to the merged inputs.
+    requires uf1.Valid()
+    requires uf2.Valid()
+    requires forward_conn.Valid()
+    requires forward_conn.i_width == uf2.input_width
+    requires forward_conn.o_width == uf1.output_width
+    ensures internal_conn.connections.Values == forward_conn.connections.Values
+    ensures forall i_index :: i_index in internal_conn.connections.Keys ==> i_index >= uf1.input_width
+    ensures forall o_index :: o_index in internal_conn.connections.Values ==> o_index < uf1.output_width
+    ensures internal_conn.Valid()
+  {
+    var internal_conn := ForwardConnectionToInternalConnectionImpl(uf1, uf2, forward_conn);
+    var i_width := internal_conn.i_width;
+    var ni_width := internal_conn.ni_width;
+    var o_width := internal_conn.o_width;
+    var nio2i := internal_conn.nio2i;
+    var connections := internal_conn.connections;
+    var i2ni := internal_conn.i2ni;
+
+    assert internal_conn.BasicValid();
+    assert internal_conn.ToNIMapValid() by {
+      reveal InternalConnection.ToNIMapValid();
+      reveal NewI2NI();
+      reveal NewNIO2I();
+    }
+    InternalConnectionToIMapValid(uf1, uf2, forward_conn);
+    assert internal_conn.ConnectionsValid() by {
+      reveal InternalConnection.ConnectionsValid();
+      reveal NewConnections();
+      assert (forall index: nat :: index in connections.Values ==> index < o_width);
+      assert (forall index: nat :: index in connections.Keys ==> index < i_width);
+    }
+    reveal InternalConnection.ConnectionsValid();
+    NewConnectionsProperties(uf1.input_width, uf1.output_width, forward_conn.connections);
+    internal_conn
+  }
+
+  opaque function ForwardConnectionModifierImpl(
+      z1: ScufInserter, z2: ScufInserter, conn: InternalConnection): (z: ScufInserter)
+    requires z1.Valid()
+    requires z2.Valid()
+    requires conn.Valid()
+    requires conn.i_width == z2.uf.input_width
+    requires conn.o_width == z1.uf.output_width
+    ensures z.Valid()
+  {
+    reveal Seq.ToSet();
+    reveal ScufInserter.Valid();
+
+    var z_par := MergeModifier(z1, z2);
+
+    var internal_conn := ForwardConnectionToInternalConnection(z1.uf, z2.uf, conn);
+
+    assert InserterConnectionConsistent(z_par, internal_conn) by {
+      assert UFConnectionConsistent(z_par.uf, internal_conn) by {
+        assert (internal_conn.i_width == z_par.uf.input_width);
+        assert (internal_conn.o_width == z_par.uf.output_width);
+      }
+      forall c: Circuit | c.Valid()
+        ensures
+          var (new_c, s) := z_par.fn(c);
+          && new_c.Valid() && s.Valid(new_c)
+          && ScufConnectionConsistent(new_c, s, internal_conn)
+      {
+        var (new_c, s) := z_par.fn(c);
+        assert z_par.Valid();
+        z_par.ValidForCircuit(c);
+        reveal SimpleInsertion();
+        assert new_c.Valid();
+        //ForwardConnectionScufConnectionConsistent(c);
+        assert ScufConnectionConsistent(new_c, s, internal_conn) by {
+          reveal ScufConnectionConsistent();
+          assert (internal_conn.i_width == s.uf.input_width);
+          assert (internal_conn.o_width == s.uf.output_width);
+          MergeModifierPathConstraints(z1, z2, c);
+          var outputs_from_s1 := Seq.ToSet(s.mp.outputs[..z1.uf.output_width]);
+          var inputs_to_s2 := Seq.ToSet(s.mp.inputs[z1.uf.input_width..]);
+          assert !PathExistsBetweenNPSets(new_c, outputs_from_s1, inputs_to_s2);
+          var conn_outputs := internal_conn.GetConnectedOutputs(s.mp);
+          var conn_inputs := internal_conn.GetConnectedInputs(s.mp);
+          assert forall o_index :: o_index in internal_conn.connections.Values
+                   ==> o_index < z1.uf.output_width by {
+            reveal InternalConnection.ConnectionsValid();
+          }
+          assert conn_outputs <= outputs_from_s1;
+          assert forall i_index :: i_index in internal_conn.connections.Keys
+                   ==> z1.uf.input_width <= i_index < z1.uf.input_width + z2.uf.input_width by {
+            reveal InternalConnection.ConnectionsValid();
+          }
+          assert conn_inputs <= inputs_to_s2;
+          NoPathExistsBetweenNPSubSets(new_c, outputs_from_s1, inputs_to_s2, conn_outputs, conn_inputs);
+          assert !PathExistsBetweenNPSets(new_c, conn_outputs, conn_inputs);
+          forall i_index | i_index in internal_conn.connections
+            ensures s.mp.inputs[i_index] !in new_c.PortSource
+          {
+            InputsOfIslandNotInPortSource(new_c, s); 
+            assert s.mp.inputs[i_index] !in new_c.PortSource;
+          }
+        }
+      }
+      reveal InserterConnectionConsistent();
+    }
+
+    var z_connected := ConnectModifier(z_par, internal_conn);
+    assert z_connected.Valid();
+    z_connected
+  }
+
+  lemma ForwardConnectBaseUFIsImplUF(z1: ScufInserter, z2: ScufInserter, conn: InternalConnection)
+    requires z1.Valid()
+    requires z2.Valid()
+    requires conn.Valid()
+    requires conn.i_width == z2.uf.input_width
+    requires conn.o_width == z1.uf.output_width
+    ensures
+      reveal ScufInserter.Valid();
+      ForwardConnectionModifierImpl(z1, z2, conn).uf == ForwardConnectBaseUF(z1.uf, z2.uf, conn)
+  {
+    reveal ScufInserter.Valid();
+    reveal ForwardConnectionModifierImpl();
+  }
+
+  function ForwardConnectBaseUF(uf1: UpdateFunction, uf2: UpdateFunction, conn: InternalConnection): (uf: UpdateFunction)
+    requires uf1.Valid()
+    requires uf2.Valid()
+    requires conn.Valid()
+    requires conn.i_width == uf2.input_width
+    requires conn.o_width == uf1.output_width
+    ensures uf.Valid()
+  {
+    var uf_par := MergeUpdateFunctions(uf1, uf2);
+    var internal_connection := ForwardConnectionToInternalConnection(uf1, uf2, conn);
+    var uf_connect := ConnectUpdateFunction(uf_par, internal_connection);
+    uf_connect
+  }
+
+  lemma ForwardConnectionUFEquivInternal(uf1: UpdateFunction, uf2: UpdateFunction, forward_conn: InternalConnection, si: SI)
+    requires uf1.Valid()
+    requires uf2.Valid()
+    requires forward_conn.Valid()
+    requires forward_conn.i_width == uf2.input_width
+    requires forward_conn.o_width == uf1.output_width
+    requires 
+      var new_uf := ForwardConnectUF(uf1, uf2, forward_conn);
+      new_uf.SIVal(si)
+    ensures 
+      var uf_base := ForwardConnectBaseUF(uf1, uf2, forward_conn);
+      var new_uf := ForwardConnectUF(uf1, uf2, forward_conn);
+      && uf_base.sf.requires(si)
+      && (new_uf.sf(si) == uf_base.sf(si))
+    {
+      var new_uf := ForwardConnectUF(uf1, uf2, forward_conn);
+      var si1 := SI(si.inputs[..uf1.input_width], si.state[..uf1.state_width]);
+      reveal UpdateFunction.Valid();
+      var so1 := uf1.sf(si1);
+      var sni2_inputs := si.inputs[uf1.input_width..];
+      var si2_inputs := forward_conn.NIO2I(sni2_inputs, so1.outputs);
+      var si2 := SI(si2_inputs, si.state[uf1.state_width..]);
+      var so2 := uf2.sf(si2);
+      var so := SO(so1.outputs + so2.outputs, so1.state + so2.state);
+      assert so == new_uf.sf(si);
+
+      var si_expanded := SI(si1.inputs + si2.inputs, si.state);
+
+      var uf_par := MergeUpdateFunctions(uf1, uf2);
+      assert so == uf_par.sf(si_expanded) by {
+        reveal MergeUpdateFunctions();
+      }
+      var internal_connection := ForwardConnectionToInternalConnection(uf1, uf2, forward_conn);
+      var uf_connect := ConnectUpdateFunction(uf_par, internal_connection);
+
+      assert uf_connect.sf(si) == internal_connection.SNI2SOSecondPass(uf_par, si) by {
+        reveal ConnectUpdateFunction();
+      }
+
+      // Following the logic inside SNI2SOSecondPass
+      var so_first_pass := internal_connection.SNI2SOFirstPass(uf_par, si);
+      var fake_output := seq(uf_par.output_width, (index: nat) requires index < uf_par.output_width => false);
+      assert so_first_pass == internal_connection.SNI2SOFromOutputs(uf_par, si, fake_output);
+      assert so_first_pass.outputs[..uf1.output_width] == so1.outputs by {
+        var si_with_fake := internal_connection.SNI2SIFromOutputs(si, fake_output);
+        assert si_with_fake.inputs == internal_connection.NIO2I(si.inputs, fake_output);
+        forall index: nat | index < uf1.input_width
+          ensures si_with_fake.inputs[index] == si1.inputs[index]
+        {
+          NewNIO2IProperties(uf1.input_width, uf2.input_width, forward_conn.nio2i, index);
+          assert si_with_fake.inputs[index] == si1.inputs[index];
+        }
+        assert si_with_fake.inputs[..uf1.input_width] == si1.inputs;
+        reveal UpdateFunction.Valid();
+        reveal MergeUpdateFunctions();
+        var so := uf_par.sf(si_with_fake);
+      }
+
+      var si_second_pass := internal_connection.SNI2SIFromOutputs(si, so_first_pass.outputs);
+      assert si_second_pass == si_expanded by {
+        forall index: nat | index < uf1.input_width + uf2.input_width
+          ensures si_second_pass.inputs[index] == si_expanded.inputs[index]
+        {
+          NewNIO2IProperties(uf1.input_width, uf2.input_width, forward_conn.nio2i, index);
+          if index < uf1.input_width {
+            assert si_second_pass.inputs[index] == si_expanded.inputs[index];
+          } else {
+            assert si_expanded.inputs[index] == forward_conn.NIO2I(sni2_inputs, so1.outputs)[index- uf1.input_width];
+            assert si_second_pass.inputs[index] == internal_connection.NIO2I(si.inputs, so_first_pass.outputs)[index];
+            var (forward_from_output, forward_index) := forward_conn.nio2i[index-uf1.input_width];
+            reveal InternalConnection.ToIMapValid();
+            if forward_from_output {
+              assert forward_index < |so_first_pass.outputs|;
+            } else {
+              assert forward_index < forward_conn.ni_width;
+            }
+            assert internal_connection.nio2i[index] ==
+              (if forward_from_output then hack(true, forward_index) else hack(false, forward_index + uf1.input_width));
+            assert si_second_pass.inputs[index] ==
+              (if forward_from_output then so_first_pass.outputs[forward_index] else si.inputs[forward_index + uf1.input_width]);
+            reveal NewNIO2I();
+            assert si_second_pass.inputs[index] == si_expanded.inputs[index];
+          }
+        }
+      }
+      reveal UpdateFunction.Valid();
+      assert uf_connect.sf(si) == uf_par.sf(si_second_pass);
+
+      assert so == uf_connect.sf(si);
+    }
+
+  lemma ForwardConnectionUFEquiv(uf1: UpdateFunction, uf2: UpdateFunction, conn: InternalConnection)
+    requires uf1.Valid()
+    requires uf2.Valid()
+    requires conn.Valid()
+    requires conn.i_width == uf2.input_width
+    requires conn.o_width == uf1.output_width
+    ensures 
+      var uf_base := ForwardConnectBaseUF(uf1, uf2, conn);
+      var new_uf := ForwardConnectUF(uf1, uf2, conn);
+      UpdateFunctionsEquiv(new_uf, uf_base)
+  {
+    var uf_base := ForwardConnectBaseUF(uf1, uf2, conn);
+    var new_uf := ForwardConnectUF(uf1, uf2, conn);
+    assert UpdateFunctionsEquiv(new_uf, uf_base) by {
+      forall si: SI | new_uf.SIVal(si)
+        ensures
+          && uf_base.sf.requires(si)
+          && (new_uf.sf(si) == uf_base.sf(si))
+      {
+        ForwardConnectionUFEquivInternal(uf1, uf2, conn, si);
+        assert new_uf.sf(si) == uf_base.sf(si);
+      }
+      reveal UpdateFunctionsEquiv();
+    }
+  }
+
+  function ForwardConnectionModifier(
+      z1: ScufInserter, z2: ScufInserter, conn: InternalConnection): (z: ScufInserter)
+    requires z1.Valid()
+    requires z2.Valid()
+    requires conn.Valid()
+    requires conn.i_width == z2.uf.input_width
+    requires conn.o_width == z1.uf.output_width
+    ensures z.Valid()
+  {
+    reveal Seq.ToSet();
+    reveal ScufInserter.Valid();
+
+    var z_conn := ForwardConnectionModifierImpl(z1, z2, conn);
+    var new_uf := ForwardConnectUF(z1.uf, z2.uf, conn);
+    assert UpdateFunctionsEquiv(new_uf, z_conn.uf) by {
+      ForwardConnectionUFEquiv(z1.uf, z2.uf, conn);
+      ForwardConnectBaseUFIsImplUF(z1, z2, conn);
+    }
+    var z := SwitchUFModifier(z_conn, new_uf);
+    z
+  }
+}
